Compile codatatypes to JavaScript. Added explicit list of non-Dafny C# and JavaScript keywords as identifiers need need IdProtect. Added create_Ctor methods in C# compilation as a more concise way to construct datatype values. Prettied up printing of codatatype values. Recognize codatatype enumerations as all-finite-values.

Binaries/DafnyRuntime.cs
@@ -770,16 +770,16 @@ namespace Dafny
         }
       }
     }
-    public Set<@_System.@__tuple_h2<U, V>> Items {
+    public Set<_System.@__tuple_h2<U, V>> Items {
       get {
-        HashSet<@_System.@__tuple_h2<U, V>> result = new HashSet<@_System.@__tuple_h2<U, V>>();
+        HashSet<_System.@__tuple_h2<U, V>> result = new HashSet<_System.@__tuple_h2<U, V>>();
         if (hasNullValue) {
-          result.Add(new @_System.@__tuple_h2<U, V>(new @_System.@__tuple_h2____hMake2<U, V>(default(U), nullValue)));
+          result.Add(_System.@__tuple_h2<U, V>.create____hMake2(default(U), nullValue));
         }
         foreach (KeyValuePair<U, V> kvp in dict) {
-          result.Add(new @_System.@__tuple_h2<U, V>(new @_System.@__tuple_h2____hMake2<U, V>(kvp.Key, kvp.Value)));
+          result.Add(_System.@__tuple_h2<U, V>.create____hMake2(kvp.Key, kvp.Value));
         }
-        return Dafny.Set<@_System.@__tuple_h2<U, V>>.FromCollection(result);
+        return Dafny.Set<_System.@__tuple_h2<U, V>>.FromCollection(result);
       }
     }
   }
@@ -1337,44 +1337,44 @@ namespace Dafny
 namespace @_System
 {
 
-  public abstract class Base___tuple_h2<@T0, @T1> { }
-  public class __tuple_h2____hMake2<@T0, @T1> : Base___tuple_h2<@T0, @T1>
+  public abstract class Base___tuple_h2<T0, T1> { }
+  public class __tuple_h2____hMake2<T0, T1> : Base___tuple_h2<T0, T1>
   {
-    public readonly @T0 @_0;
-    public readonly @T1 @_1;
-    public __tuple_h2____hMake2(@T0 @_0, @T1 @_1)
+    public readonly T0 _0;
+    public readonly T1 _1;
+    public __tuple_h2____hMake2(T0 _0, T1 _1)
     {
-      this.@_0 = @_0;
-      this.@_1 = @_1;
+      this._0 = _0;
+      this._1 = _1;
     }
     public override bool Equals(object other)
     {
-      var oth = other as _System.@__tuple_h2____hMake2<@T0, @T1>;
-      return oth != null && this.@_0.Equals(oth.@_0) && Dafny.Helpers.AreEqual(this.@_1, oth.@_1);
+      var oth = other as _System.@__tuple_h2____hMake2<T0, T1>;
+      return oth != null && this._0.Equals(oth._0) && Dafny.Helpers.AreEqual(this._1, oth._1);
     }
     public override int GetHashCode()
     {
       ulong hash = 5381;
       hash = ((hash << 5) + hash) + 0;
-      hash = ((hash << 5) + hash) + ((ulong)Dafny.Helpers.GetHashCode(this.@_0));
-      hash = ((hash << 5) + hash) + ((ulong)Dafny.Helpers.GetHashCode(this.@_1));
+      hash = ((hash << 5) + hash) + ((ulong)Dafny.Helpers.GetHashCode(this._0));
+      hash = ((hash << 5) + hash) + ((ulong)Dafny.Helpers.GetHashCode(this._1));
       return (int)hash;
     }
     public override string ToString()
     {
       string s = "";
       s += "(";
-      s += Dafny.Helpers.ToString(this.@_0);
+      s += Dafny.Helpers.ToString(this._0);
       s += ", ";
-      s += Dafny.Helpers.ToString(this.@_1);
+      s += Dafny.Helpers.ToString(this._1);
       s += ")";
       return s;
     }
   }
-  public struct @__tuple_h2<@T0, @T1>
+  public struct __tuple_h2<T0, T1>
   {
-    Base___tuple_h2<@T0, @T1> _d;
-    public Base___tuple_h2<@T0, @T1> _D
+    Base___tuple_h2<T0, T1> _d;
+    public Base___tuple_h2<T0, T1> _D
     {
       get
       {
@@ -1384,26 +1384,29 @@ namespace @_System
         return _d;
       }
     }
-    public @__tuple_h2(Base___tuple_h2<@T0, @T1> d) { this._d = d; }
-    static Base___tuple_h2<@T0, @T1> theDefault;
-    public static Base___tuple_h2<@T0, @T1> Default
+    public __tuple_h2(Base___tuple_h2<T0, T1> d) { this._d = d; }
+    static Base___tuple_h2<T0, T1> theDefault;
+    public static Base___tuple_h2<T0, T1> Default
     {
       get
       {
         if (theDefault == null) {
-          theDefault = new _System.@__tuple_h2____hMake2<@T0, @T1>(default(@T0), default(@T1));
+          theDefault = new _System.@__tuple_h2____hMake2<T0, T1>(default(T0), default(T1));
         }
         return theDefault;
       }
     }
     public override bool Equals(object other)
     {
-      return other is @__tuple_h2<@T0, @T1> && _D.Equals(((@__tuple_h2<@T0, @T1>)other)._D);
+      return other is __tuple_h2<T0, T1> && _D.Equals(((__tuple_h2<T0, T1>)other)._D);
     }
     public override int GetHashCode() { return _D.GetHashCode(); }
     public override string ToString() { return _D.ToString(); }
-    public bool is____hMake2 { get { return _D is __tuple_h2____hMake2<@T0, @T1>; } }
-    public @T0 dtor__0 { get { return ((__tuple_h2____hMake2<@T0, @T1>)_D).@_0; } }
-    public @T1 dtor__1 { get { return ((__tuple_h2____hMake2<@T0, @T1>)_D).@_1; } }
+    public static __tuple_h2<T0,T1> create____hMake2(T0 _0, T1 _1) {
+      return new __tuple_h2<T0,T1>(new __tuple_h2____hMake2<T0,T1>(_0, _1));
+    }
+    public bool is____hMake2 { get { return _D is __tuple_h2____hMake2<T0, T1>; } }
+    public T0 dtor__0 { get { return ((__tuple_h2____hMake2<T0, T1>)_D)._0; } }
+    public T1 dtor__1 { get { return ((__tuple_h2____hMake2<T0, T1>)_D)._1; } }
   }
 } // end of namespace _System
