Test/js/Dt.dfy
@@ -2,7 +2,7 @@
 // RUN: %dafny /compile:3 /spillTargetCode:2 /compileTarget:js "%s" >> "%t"
 // RUN: %diff "%s.expect" "%t"
 
-datatype Dt = Nil | Cons(head: int, tail: Dt)
+datatype List = Nil | Cons(head: int, tail: List)
 
 method Main() {
   var a := Nil;
@@ -25,32 +25,87 @@ method Main() {
   print " == ", s;
   s := SumAgain(u);
   print " (once more, that's ", s, ")\n";
+
+  CoDt();
+  AllBerry();
 }
 
-function method Up(m: nat, n: nat): Dt
+function method Up(m: nat, n: nat): List
   requires m <= n
   decreases n - m
 {
   if m == n then Nil else Cons(m, Up(m+1, n))
 }
 
-function method Sum(xs: Dt): int {
+function method Sum(xs: List): int {
   match xs  // top-level match expression
   case Nil => 0
   case Cons(x, tail) => x + Sum(tail)
 }
 
-function method SumAgain(xs: Dt): int {
+function method SumAgain(xs: List): int {
   var r := match xs  // let expression; non-top-level match expression
     case Nil => 0
     case Cons(x, tail) => x + SumAgain(tail);
   r
 }
 
-method PrintSum(xs: Dt, prefix: string) {
+method PrintSum(xs: List, prefix: string) {
   match xs  // match statement
   case Nil =>
   case Cons(x, tail) =>
     print prefix, x;
     PrintSum(tail, " + ");  // tail recursion
+}
+
+method CoDt() {
+  var s := CoUp(0, true);
+  var l := ToList(s, 4);
+  print l, "\n";
+  if l.Cons? {
+    print l.head, " ", l.tail, "\n";
+  }
+  print s, "\n";
+  var s' := Next(-20, s);  // not a lazy invocation
+  print s', "\n";
+}
+
+codatatype Stream = Next(shead: int, stail: Stream)
+
+function method CoUp(n: int, b: bool): Stream
+{
+  if b then
+    CoUp(n, false)  // recursive, not co-recursive, call
+  else
+    Next(n, CoUp(n+1, true))  // CoUp is co-recursive call
+}
+
+function method ToList(s: Stream, n: nat): List
+{
+  if n == 0 then Nil else Cons(s.shead, ToList(s.stail, n-1))
+}
+
+datatype Berry = Smultron | Jordgubb | Hjortron | Hallon
+predicate method IsRed(b: Berry) {
+  b != Berry.Hjortron
+}
+
+codatatype CoBerry = Smultron | Jordgubb | Hjortron | Hallon  // no reason for this to be a co-datatype, but, hey, why not
+predicate method IsCoRed(b: CoBerry) {
+  b == CoBerry.Hjortron
+}
+
+method AllBerry() {
+  var s := set b: Berry | IsRed(b);
+  print s, "\n";
+  var c :| IsCoRed(c);
+  print c, " ", c.Hjortron?, " ", c == CoBerry.Hjortron, " ", c.Smultron?, "\n";
+  var n := Inf();
+  print n == Zero, "\n";
+}
+
+codatatype NatPlus = Succ(NatPlus) | Zero
+
+function method Inf(): NatPlus {
+  Succ(Inf())
 }
